Message header serialization
Move separate logical entities into their respective modules and split up the file.
Started serialization implementation.

Made map on sequences generic, added flatten, minor cosmetic changes

WIP: msg header serialization

Implemented up to typ (so just first two fields of header body)

Changed post-condition of WriteSingleByte, work-around for Dafny bug

Verification, including UTF8 validity of KV pairs takes around 1 min

WIP: Added algorithm suite ID serialization

WIP: serialization performing terribly

WIP: temp commit before array->seq rewrite in stream

Added check for aliasing (thanks to Sam's help)

Implemented, but not verified AAD serialization

WIP: added EDK serialization, verification errors, but no timeouts

added assume false for AAD and HeaderBody

WIP: Implemented serialization with assume false

Added post-condition to deserialization, but times out

We need to establish freshness. I've added invariants and post-conditions to deserialization but they time out.

WIP: some trials with adding fresh

WIP: moving assume false past AAD works and code cleanup

WIP: trying to make serialziation of header body work

using opaque on validity predicates and repr functions, failing after serializeAAD right now

refactored aad and edk serialization into their own files.

WIP: Towards verification of Serialize.dfy

Dafny not timing out anymore, but not correctly verifying yet.

Using Dafny without HeapSucc transitivity axiom and with the -arith:8 flag
which both help.

ReprAAD is opaque, but then Validity.dfy not verifying.
If it is transparent, verification slows down.

serializeAADImpl/serializeEDKImpl not maintaining the old state of os.data

WIP: Serialize.dfy verifying in ~3min

WIP: simplified Serialize.dfy verification and cleanup

reveal ReprAAD()

src/StandardLibrary/StandardLibrary.dfy
@@ -7,7 +7,7 @@ module {:extern "STL"} StandardLibrary {
 
   datatype Either<S,T> = Left(left: S) | Right(right: T)
 
-  datatype Error = IOError(msg: string) | DeserializationError(msg: string)
+  datatype Error = IOError(msg: string) | DeserializationError(msg: string) | SerializationError(msg: string)
 
   type Result<T> = Either<T, Error>
 
@@ -250,13 +250,23 @@ module {:extern "STL"} StandardLibrary {
       }
     }
 
-  function method seq_map<S, T>(s : seq<S>, f : S -> T) : seq<T> {
-    if s == [] then [] else
-    [f(s[0])] + seq_map(s[1..], f)
+  function method MapSeq<S, T>(s: seq<S>, f: S ~> T): seq<T>
+    requires forall i :: 0 <= i < |s| ==> f.requires(s[i])
+    reads set i,o | 0 <= i < |s| && o in f.reads(s[i]) :: o
+  {
+      if s == []
+      then []
+      else [f(s[0])] + MapSeq(s[1..], f)
+  }
+
+  function method FlattenSeq<T>(s: seq<seq<T>>): seq<T> {
+      if s == []
+      then []
+      else s[0] + FlattenSeq(s[1..])
   }
 
   predicate method uniq_fst<S(==), T(==)> (s : seq<(S, T)>) {
-    uniq(seq_map(s, (x : (S, T)) => x.0))
+    uniq(MapSeq(s, (x : (S, T)) => x.0))
   }
 
 
