src/Util/Streams.dfy
@@ -8,28 +8,32 @@ module Streams {
 
     ghost var Repr : set<object>
     predicate Valid() reads this
-    function method capacity() : nat reads this requires Valid() // An upper bound on the amount of data the stream can accept on Write
+    function method capacity()  : nat reads this requires Valid() // An upper bound on the amount of data the stream can accept on Write
     function method available() : nat reads this requires Valid() // An upper bound on the amount of data the stream can deliver on Read
 
 
-    method Write(a : array<uint8>, off : nat, req : nat) returns (len_written : Either<nat, Error>)
+    method Write(a : array<uint8>, off : nat, req : nat) returns (res : Either<nat, Error>)
       requires Valid()
       requires a.Length >= off + req
       modifies Repr
       requires a !in Repr
-      ensures len_written.Left? ==> len_written.left == min(req, old(capacity()))
-      ensures len_written.Right? ==> unchanged(this)
       ensures Valid()
+      ensures
+        match res
+          case Left(len_written) => len_written == min(req, old(capacity()))
+          case Right(e) => true
 
 
-    method Read(i : array<uint8>, off : nat, req : nat) returns (len_read : Either<nat, Error>)
+    method Read(i : array<uint8>, off : nat, req : nat) returns (res : Either<nat, Error>)
       requires Valid()
       requires i.Length >= off + req
       requires i !in Repr
       modifies i, this
       ensures Valid()
-      ensures len_read.Left? ==> len_read.left == min(req, old(available())) 
-      ensures len_read.Right? ==> unchanged(this)
+      ensures
+        match res
+          case Left(len_read) => len_read == min(req, old(available()))
+          case Right(e) => true
   }
 
 
@@ -56,34 +60,36 @@ module Streams {
         pos := 0;
     }
 
-    method Write(a : array<uint8>, off : nat, req : nat) returns (len_written : Either<nat, Error>)
+    method Write(a : array<uint8>, off : nat, req : nat) returns (res : Either<nat, Error>)
       requires Valid()
       modifies this
       requires a !in Repr
-      ensures len_written.Left? ==> len_written.left == min(req, old(capacity()))
-      ensures len_written.Right? ==> unchanged(this)
       ensures Valid()
-      ensures len_written.Right?
+      ensures
+        match res
+          case Left(len_written) => len_written == min(req, old(capacity()))
+          case Right(e) => unchanged(this)
     {
-      len_written := Right(IOError("Cannot write to StringReader"));
+      res := Right(IOError("Cannot write to StringReader"));
     }
     
-    method Read(arr : array<uint8>, off : nat, req : nat) returns (len_read : Either<nat, Error>)
+    method Read(arr : array<uint8>, off : nat, req : nat) returns (res : Either<nat, Error>)
       requires Valid()
       requires arr.Length >= off + req
       requires arr != data
       ensures Valid()
       modifies arr, this
-      ensures len_read.Left? ==> len_read.left == min(req, old(available())) 
-      ensures len_read.Right? ==> unchanged(this) && unchanged(arr)
       ensures unchanged(`data)
       ensures var n := min(req, old(available()));
         arr[..] == arr[..off] + data[old(pos) .. (old(pos) + n)] + arr[off + n ..]
-      ensures len_read.Left?
+      ensures
+        match res
+          case Left(len_read) => len_read == min(req, old(available()))
+          case Right(e) => unchanged(this) && unchanged(arr)
     {
       if off == arr.Length || available() == 0 {
         assert (min (req, available())) == 0;
-        len_read := Left(0);
+        res := Left(0);
       }
       else {
         var n := min(req, available());
@@ -91,71 +97,193 @@ module Streams {
           arr[off + i] := data[pos + i];
         }
         pos := pos + n;
-        len_read := Left(n);
+        res := Left(n);
       }
     }
+    /*
+    // TODO add a version without arrays
+    method ReadSimple(arr: array<uint8>) returns (res: Result<nat>)
+      requires Valid()
+      ensures Valid()
+      modifies this
+      ensures
+        match res
+          case Left(len_read) =>
+            var n := arr.Length;
+            && pos == old(pos) + n
+            && arr[..] == data[old(pos) .. pos]
+            && len_read == n
+          case Right(e) => unchanged(this)
+    {
+      if arr.Length <= available() {
+        forall i | 0 <= i < arr.Length {
+          arr[i] := data[pos + i];
+        }
+        pos := pos + arr.Length;
+        res := Left(arr.Length);
+      } else {
+        res := Right(IOError("Not enough bytes available on stream."));
+      }
+    }
+    */
   }
 
   class StringWriter extends Stream {
-    var data : array<uint8>
-    var pos : nat
+    ghost var data : seq<uint8>
 
-    predicate Valid() reads this {
-      this in Repr &&
-      data in Repr &&
-      pos <= data.Length 
+    predicate Valid()
+      reads this
+    {
+      this in Repr
     }
 
-    function method capacity() : nat reads this requires Valid() { data.Length - pos }
-    function method available() : nat reads this requires Valid() { 0 }
+    function method capacity(): nat
+      reads this
+      requires Valid() 
 
+    function method available(): nat
+      reads this
+      requires Valid()
 
     constructor(n : nat)
       ensures Valid()
     {
-        data := new uint8[n];
-        Repr := {this, data};
-        pos := 0;
+        data := [];
+        Repr := {this};
     }
-
-    method Write(a : array<uint8>, off : nat, req : nat) returns (len_written : Either<nat, Error>)
+    
+    method Write(a: array<uint8>, off: nat, req: nat) returns (res: Result<nat>)
       requires Valid()
-      requires a.Length >= off + req
-      modifies this, data
+      requires off + req <= a.Length
       requires a !in Repr
-      ensures len_written.Left? ==> len_written.left == min(req, old(capacity()))
-      ensures len_written.Right? ==> unchanged(this)
+      modifies `data
+      ensures unchanged(`Repr)
       ensures Valid()
-      ensures unchanged(`data)
-      ensures var n := min(req, old(capacity()));
-        data[..] == old(data)[..old(pos)] + a[off .. off + n] + old(data)[old(pos) + n ..]
-      ensures len_written.Left?
+      ensures
+        match res
+          case Left(len_written) =>
+            if old(capacity()) == 0
+            then
+              len_written == 0
+            else
+              //&& old(pos + n < |data|)
+              //&& Written(old(data), data, old(pos), pos, a[off..off+n], len_written, n)
+              && len_written == min(req, old(capacity()))
+              && data == old(data) + a[off..off+req]
+          case Right(e) => true
     {
       if off == a.Length || capacity() == 0 {
-        len_written := Left(0);
+        res := Left(0);
       }
       else {
         var n := min(req, capacity());
-        forall i | 0 <= i < min(req, capacity()) {
-          data[pos + i] := a[off + i];
-        }
-        len_written := Left(n);
-        pos := pos + n;
+        data := data + a[off..off+req];
+        res := Left(n);
+      }
+    }
 
+    method WriteSimple(a: array<uint8>) returns (res: Result<nat>)
+      requires Valid()
+      requires a !in Repr
+      modifies `data
+      ensures unchanged(`Repr)
+      ensures unchanged(a)
+      ensures Valid()
+      ensures
+        match res
+          case Left(len_written) =>
+              && len_written == a.Length
+              && data[..] == old(data) + a[..]
+          case Right(e) => unchanged(`data)
+    {
+      if a.Length <= capacity() {
+        data := data + a[..];
+        res := Left(a.Length);
+      } else {
+        res := Right(IOError("Reached end of stream."));
+      }
+    }
+
+    method WriteSimpleSeq(a: seq<uint8>) returns (res: Result<nat>)
+      requires Valid()
+      modifies `data
+      ensures unchanged(`Repr)
+      ensures Valid()
+      ensures
+        match res
+          case Left(len_written) =>
+              && len_written == |a|
+              && data[..] == old(data) + a
+          case Right(e) => unchanged(`data)
+    {
+      if |a| <= capacity() {
+        data := data + a;
+        res := Left(|a|);
+      } else {
+        res := Right(IOError("Reached end of stream."));
+      }
+    }
+
+    method WriteSingleByte(a: uint8) returns (res: Result<nat>)
+      requires Valid()
+      modifies `data
+      ensures unchanged(`Repr)
+      ensures Valid()
+      ensures
+        match res
+          case Left(len_written) => 
+            if old(capacity()) == 0
+            then
+              len_written == 0
+            else 
+              && len_written == 1
+              && data == old(data) + [a]
+              // Dafny->Boogie drops an old: https://github.com/dafny-lang/dafny/issues/320
+              //&& data[..] == old(data)[.. old(pos)] + [a] + old(data)[old(pos) + 1 ..]
+          case Right(e) => unchanged(`data)
+    {
+      if capacity() == 0 {
+        res := Left(0);
+      }
+      else {
+        data := data + [a];
+        res := Left(1);
+      }
+    }
+
+    method WriteSingleByteSimple(a: uint8) returns (res: Result<nat>)
+      requires Valid()
+      modifies `data
+      ensures unchanged(`Repr)
+      ensures Valid()
+      ensures
+        match res
+          case Left(len_written) =>
+              len_written == 1
+              && data == old(data) + [a]
+              // Dafny->Boogie drops an old: https://github.com/dafny-lang/dafny/issues/320
+              //&& data[..] == old(data)[.. old(pos)] + [a] + old(data)[old(pos) + 1 ..]
+          case Right(e) => unchanged(`data)
+    {
+      if 1 <= capacity() {
+        data := data + [a];
+        res := Left(1);
+      } else {
+        res := Right(IOError("Reached end of stream."));
       }
     }
     
-    method Read(arr : array<uint8>, off : nat, req : nat) returns (len_read : Either<nat, Error>)
+    method Read(arr : array<uint8>, off : nat, req : nat) returns (res : Result<nat>)
       requires Valid()
       requires arr.Length >= off + req
-      requires arr != data
       ensures Valid()
       modifies arr, this
-      ensures len_read.Left? ==> len_read.left == min(req, old(available())) 
-      ensures len_read.Right? ==> unchanged(this) && unchanged(arr)
-      ensures len_read.Right?
+      ensures
+        match res
+          case Left(len_read) => len_read == min(req, old(available()))
+          case Right(e) => unchanged(this) && unchanged(arr)
     {
-      len_read := Right(IOError("Cannot read from StringWriter"));
+      res := Right(IOError("Cannot read from StringWriter"));
     }
   }
 
