src/Util/UTF8.dfy
@@ -16,75 +16,75 @@ module UTF8 {
     import opened UInt = StandardLibrary.UInt
 
     // Returns the value of the idx'th bit, from least to most significant bit (0- indexed)
-    function method bit_at (x: uint8, idx: uint8): bool
-    requires idx < 8
+    function method bit_at(x: uint8, idx: uint8): bool
+        requires idx < 8
     {
-    var w := x as bv8;
-    (w >> idx) & 1 == 1
+        var w := x as bv8;
+        (w >> idx) & 1 == 1
     }
 
     // Checks if a[offset] is a valid continuation uint8.
-    predicate method ValidUTF8Continuation (a : array<uint8>, offset : nat)
+    predicate method ValidUTF8Continuation(a: array<uint8>, offset: nat)
+        requires offset < a.Length
         reads a
-        requires a.Length > offset 
     {
             bit_at(a[offset], 7) && !bit_at(a[offset], 6)
     }
 
     // Returns which leading uint8 is at a[offset], or 0 if it is not a leading uint8.
-    function method CodePointCase (a : array<uint8>, offset: nat)  : uint8
-        reads a
+    function method CodePointCase(a: array<uint8>, offset: nat): uint8
         requires offset < a.Length
+        reads a
     {
-
-        if bit_at(a[offset], 7) then // 1xxxxxxx
-            if bit_at(a[offset], 6) then //11xxxxxx
-                if bit_at(a[offset], 5) then // 111xxxxx
-                    if bit_at(a[offset], 4) then // 1111xxxx
-                        if bit_at(a[offset], 3) then // 11111xxx
+        if bit_at(a[offset], 7) then // 1xxx xxxx
+            if bit_at(a[offset], 6) then //11xx xxxx
+                if bit_at(a[offset], 5) then // 111x xxxx
+                    if bit_at(a[offset], 4) then // 1111 xxxx
+                        if bit_at(a[offset], 3) then // 1111 1xxx
                             0 // Error case
-                        else // 11110xxx
+                        else // 1111 0xxx
                             4 
-                    else // 1110xxxx 
+                    else // 1110 xxxx 
                         3
-                else // 110xxxx
+                else // 110x xxxx
                     2
-            else //10xxxxxx
+            else //10xx xxxx
                 0 // Error case
         else //0xxxxxxx
             1
     }
 
-    predicate method ValidUTF8_at (a : array<uint8>, offset : nat)
-        reads a 
+    predicate method ValidUTF8_at(a: array<uint8>, offset: nat)
         requires offset <= a.Length
+        reads a 
         decreases (a.Length - offset)
     {
-        if offset == a.Length then true else
-        var c := CodePointCase(a, offset);
-        if c == 1 then 
-            ValidUTF8_at(a, offset + 1)
-        else if c == 2 then
-            !bit_at(a[offset], 3) && 
-            a.Length >= offset + 2 && 
-            ValidUTF8Continuation(a, offset + 1) && 
-            ValidUTF8_at(a, offset + 2)
-        else if c == 3 then
-            !bit_at(a[offset], 4) && 
-            a.Length >= offset + 3 && 
-            ValidUTF8Continuation(a, offset + 1) && 
-            ValidUTF8Continuation(a, offset + 2) && 
-            ValidUTF8_at(a, offset + 3) 
-        else  // c == 4
-            !bit_at(a[offset], 3) && 
-            a.Length >= offset + 4 && 
-            ValidUTF8Continuation(a, offset + 1) && 
-            ValidUTF8Continuation(a, offset + 2) && 
-            ValidUTF8Continuation(a, offset + 3) && 
-            ValidUTF8_at(a, offset + 4)
+        if offset == a.Length
+        then true 
+        else
+            var c := CodePointCase(a, offset);
+            if c == 1 then 
+                ValidUTF8_at(a, offset + 1)
+            else if c == 2 then
+                offset + 2 <= a.Length && 
+                ValidUTF8Continuation(a, offset + 1) && 
+                ValidUTF8_at(a, offset + 2)
+            else if c == 3 then
+                offset + 3 <= a.Length && 
+                ValidUTF8Continuation(a, offset + 1) && 
+                ValidUTF8Continuation(a, offset + 2) && 
+                ValidUTF8_at(a, offset + 3) 
+            else if c == 4 then
+                offset + 4 <= a.Length && 
+                ValidUTF8Continuation(a, offset + 1) && 
+                ValidUTF8Continuation(a, offset + 2) && 
+                ValidUTF8Continuation(a, offset + 3) && 
+                ValidUTF8_at(a, offset + 4)
+            else
+                false
     }
 
-    predicate method ValidUTF8 (a : array<uint8>)
+    predicate method ValidUTF8(a: array<uint8>)
         reads a
     {
         ValidUTF8_at(a, 0)
