src/SDK/AlgorithmSuite.dfy
@@ -9,8 +9,11 @@ module AlgorithmSuite {
   import Digests
   import S = Signature
   import opened StandardLibrary
+  import opened UInt = StandardLibrary.UInt
 
-  newtype ID = x | 0 <= x < 0x1_0000
+  const validIDs: set<uint16> := {0x0378, 0x0346, 0x0214, 0x0178, 0x0146, 0x0114, 0x0078, 0x0046, 0x0014};
+
+  newtype ID = x | x in validIDs witness 0x0014
   const AES_256_GCM_IV12_AUTH16_KDSHA384_SIGEC384 : ID := 0x0378
   const AES_192_GCM_IV12_AUTH16_KDSHA384_SIGEC384 : ID := 0x0346
   const AES_128_GCM_IV12_AUTH16_KDSHA256_SIGEC256 : ID := 0x0214
