src/SDK/MessageHeader/Definitions.dfy
@@ -1,0 +1,42 @@
+include "../AlgorithmSuite.dfy"
+include "../../StandardLibrary/StandardLibrary.dfy"
+
+module MessageHeader.Definitions {
+    import AlgorithmSuite
+    import opened StandardLibrary
+    import opened UInt = StandardLibrary.UInt
+
+    type T_NonZero_uint16  = x: uint16 | x != 0 witness 1
+    /*
+    * Header body type definition
+    */
+    type T_Version         = x | x == 0x01 /*Version 1.0*/ witness 0x01
+    type T_Type            = x | x == 0x80 /*Customer Authenticated Encrypted Data*/ witness 0x80
+    type T_MessageID       = x: seq<uint8> | |x| == 16 witness [0,0,0,0,0,0,0,0,0,0,0,0,0,0,0,0]
+    type T_Reserved        = x: seq<uint8> | x == [0,0,0,0] witness [0,0,0,0]
+    datatype T_ContentType = NonFramed | Framed
+    type EncCtx            = array<(array<uint8>, array<uint8>)>
+    datatype T_AAD         = AAD(length: T_NonZero_uint16, kvPairs: EncCtx) | EmptyAAD
+
+    datatype EDKEntry      = EDKEntry(keyProviderId: array<uint8>, keyProviderInfo: array<uint8>, encDataKey: array<uint8>)
+    datatype T_EncryptedDataKeys
+                           = EncryptedDataKeys(count: T_NonZero_uint16, entries: array<EDKEntry>)
+
+    datatype HeaderBody    = HeaderBody(
+                                version: T_Version,
+                                typ: T_Type,
+                                algorithmSuiteID: AlgorithmSuite.ID,
+                                messageID: T_MessageID,
+                                aad: T_AAD,
+                                encryptedDataKeys: T_EncryptedDataKeys,
+                                contentType: T_ContentType,
+                                reserved: T_Reserved,
+                                ivLength: uint8,
+                                frameLength: uint32)
+
+    /*
+    * Header authentication type definition
+    */
+    
+    datatype HeaderAuthentication = HeaderAuthentication(iv: array<uint8>, authenticationTag: array<uint8>)
+}
