src/SDK/MessageHeader/Deserialize.dfy
@@ -1,0 +1,620 @@
+include "Definitions.dfy"
+include "Utils.dfy"
+include "Validity.dfy"
+
+include "../AlgorithmSuite.dfy"
+include "../../Util/Streams.dfy"
+include "../../StandardLibrary/StandardLibrary.dfy"
+include "../../Util/UTF8.dfy"
+
+
+/*
+ * The message header deserialization
+ * 
+ * The message header is deserialized from a uint8 stream.
+ * When encountering an error, we stop and return it immediately, leaving the remaining inputs on the stream
+ */
+module MessageHeader.Deserialize {
+    import opened Definitions
+    import opened Validity
+    import opened Utils
+
+    import AlgorithmSuite
+    import opened Streams
+    import opened StandardLibrary
+    import opened UInt = StandardLibrary.UInt
+    import opened UTF8
+
+    /*
+     * Message header-specific
+     */
+
+    method deserializeVersion(is: StringReader) returns (ret: Result<T_Version>)
+        requires is.Valid()
+        modifies is
+        ensures is.Valid()
+    {
+        var res := readFixedLengthFromStreamOrFail(is, 1);
+        match res {
+            case Left(version) =>
+                if version[0] == 0x01 {
+                    return Left(version[0] as T_Version);
+                } else {
+                    return Right(DeserializationError("Version not supported."));
+                }
+            case Right(e) => return Right(e);
+        }
+    }
+
+    method deserializeType(is: StringReader) returns (ret: Result<T_Type>)
+        requires is.Valid()
+        modifies is
+        ensures is.Valid()
+    {
+        var res := readFixedLengthFromStreamOrFail(is, 1);
+        match res {
+            case Left(typ) =>
+                if typ[0] == 0x80 {
+                    return Left(typ[0] as T_Type);
+                } else {
+                    return Right(DeserializationError("Type not supported."));
+                }
+            case Right(e) => return Right(e);
+        }
+    }
+
+    method deserializeAlgorithmSuiteID(is: StringReader) returns (ret: Result<AlgorithmSuite.ID>)
+        requires is.Valid()
+        modifies is
+        ensures
+            match ret
+                case Left(algorithmSuiteID) => ValidAlgorithmID(algorithmSuiteID)
+                case Right(_) => true
+        ensures is.Valid()
+    {
+        var res := readFixedLengthFromStreamOrFail(is, 2);
+        match res {
+            case Left(algorithmSuiteID) =>
+                var asid := arrayToUInt16(algorithmSuiteID);
+                if asid in AlgorithmSuite.validIDs {
+                    return Left(asid as AlgorithmSuite.ID);
+                } else {
+                    return Right(DeserializationError("Algorithm suite not supported."));
+                }
+            case Right(e) => return Right(e);
+        }
+    }
+
+    // TODO:
+    predicate method isValidMsgID (candidateID: array<uint8>)
+        requires candidateID.Length == 16
+        ensures ValidMessageId(candidateID[..])
+    {
+        true
+    }
+    method deserializeMsgID(is: StringReader) returns (ret: Result<T_MessageID>)
+        requires is.Valid()
+        modifies is
+        ensures
+            match ret
+                case Left(msgId) => ValidMessageId(msgId)
+                case Right(_) => true
+        ensures is.Valid()
+    {
+        var res := readFixedLengthFromStreamOrFail(is, 16);
+        match res {
+            case Left(msgId) =>
+                if isValidMsgID(msgId) {
+                    return Left(msgId[..]);
+                } else {
+                    return Right(DeserializationError("Not a valid Message ID."));
+                }
+            case Right(e) => return Right(e);
+        }
+    }
+
+    method deserializeUTF8(is: StringReader, n: nat) returns (ret: Result<array<uint8>>)
+        requires is.Valid()
+        modifies is
+        ensures
+            match ret
+                case Left(bytes) =>
+                    && bytes.Length == n
+                    && ValidUTF8(bytes)
+                    && fresh(bytes)
+                case Right(_) => true
+        ensures is.Valid()
+    {
+        ret := readFixedLengthFromStreamOrFail(is, n);
+        match ret {
+            case Left(bytes) =>
+                if ValidUTF8(bytes) {
+                    return ret;
+                } else {
+                    return Right(DeserializationError("Not a valid UTF8 string."));
+                }
+            case Right(e) => return ret;
+        }
+    }
+
+    method deserializeUnrestricted(is: StringReader, n: nat) returns (ret: Result<array<uint8>>)
+        requires is.Valid()
+        modifies is
+        ensures
+            match ret
+                case Left(bytes) =>
+                    && bytes.Length == n
+                    && fresh(bytes)
+                case Right(_) => true
+        ensures is.Valid()
+    {
+        ret := readFixedLengthFromStreamOrFail(is, n);
+    }
+
+    // TODO: Probably this should be factored out into EncCtx at some point
+    method deserializeAAD(is: StringReader) returns (ret: Result<T_AAD>)
+        requires is.Valid()
+        modifies is
+        ensures
+            match ret
+                case Left(aad) => 
+                    && ValidAAD(aad)
+                    // TODO: I think we need to establish freshness to connect
+                    //       deserialization with the caller.
+                    //       Times out.
+                    //&& fresh(ReprAAD(aad))
+                case Right(_) => true
+        ensures is.Valid()
+    {
+        var kvPairsLength: uint16;
+        {
+            var res := deserializeUnrestricted(is, 2);
+            match res {
+                case Left(bytes) => kvPairsLength := arrayToUInt16(bytes);
+                case Right(e) => return Right(e);
+            }
+        }
+        if kvPairsLength == 0 {
+            return Left(EmptyAAD);
+        }
+        var totalBytesRead := 0;
+
+        var kvPairsCount: uint16;
+        {
+            var res := deserializeUnrestricted(is, 2);
+            match res {
+                case Left(bytes) =>
+                    kvPairsCount := arrayToUInt16(bytes);
+                    totalBytesRead := totalBytesRead + bytes.Length;
+                    if kvPairsLength > 0 && kvPairsCount == 0 {
+                        return Right(DeserializationError("Key value pairs count is 0."));
+                    }
+                    assert kvPairsLength > 0 ==> kvPairsCount > 0;
+                case Right(e) => return Right(e);
+            }
+        }
+
+        var kvPairs: EncCtx := new [kvPairsCount];
+        assert kvPairs.Length > 0;
+        assert kvPairsCount == kvPairs.Length as uint16;
+
+        var i := 0;
+        while i < kvPairsCount
+            invariant is.Valid()
+            invariant i <= kvPairsCount
+            invariant InBoundsKVPairsUpTo(kvPairs, i as nat)
+            invariant SortedKVPairsUpTo(kvPairs, i as nat)
+            invariant forall j :: 0 <= j < i ==> ValidUTF8(kvPairs[j].0)
+            invariant forall j :: 0 <= j < i ==> ValidUTF8(kvPairs[j].1)
+            // TODO: I think we need to establish freshness to connect
+            //       deserialization with the caller.
+            //       Times out.
+            //invariant fresh(ReprAADUpTo(kvPairs, i as nat))
+        {
+            var keyLength: uint16;
+            {
+                var res := deserializeUnrestricted(is, 2);
+                match res {
+                    case Left(bytes) =>
+                        keyLength := arrayToUInt16(bytes);
+                        totalBytesRead := totalBytesRead + bytes.Length;
+                    case Right(e) => return Right(e);
+                }
+            }
+
+            var key := new uint8[keyLength];
+            {
+                var res := deserializeUTF8(is, keyLength as nat);
+                match res {
+                    case Left(bytes) =>
+                        key := bytes;
+                        totalBytesRead := totalBytesRead + bytes.Length;
+                    case Right(e) => return Right(e);
+                }
+            }
+            assert key.Length <= UINT16_MAX;
+
+            var valueLength: uint16;
+            {
+                var res := deserializeUnrestricted(is, 2);
+                match res {
+                    case Left(bytes) =>
+                        valueLength := arrayToUInt16(bytes);
+                        totalBytesRead := totalBytesRead + bytes.Length;
+                    case Right(e) => return Right(e);
+                }
+            }
+
+            var value := new uint8[valueLength];
+            {
+                var res := deserializeUTF8(is, valueLength as nat);
+                match res {
+                    case Left(bytes) =>
+                        value := bytes;
+                        totalBytesRead := totalBytesRead + bytes.Length;
+                    case Right(e) => return Right(e);
+                }
+            }
+            assert value.Length <= UINT16_MAX;
+            
+            // check for sortedness by key
+            if i > 0 {
+                if lexCmpArrays(kvPairs[i-1].0, key, ltByte) {
+                    kvPairs[i] := (key, value);
+                } else {
+                    return Right(DeserializationError("Key-value pairs must be sorted by key."));
+                }
+            } else {
+                assert i == 0;
+                kvPairs[i] := (key, value);
+            }
+            assert SortedKVPairsUpTo(kvPairs, (i+1) as nat);
+            i := i + 1;
+        }
+        if (kvPairsLength as nat) != totalBytesRead {
+            return Right(DeserializationError("Bytes actually read differs from bytes supposed to be read."));
+        }
+        return Left(AAD(kvPairsLength, kvPairs));
+    }
+
+    // TODO: Probably this should be factored out into EDK at some point
+    method deserializeEncryptedDataKeys(is: StringReader, ghost aad: T_AAD) returns (ret: Result<T_EncryptedDataKeys>)
+        requires is.Valid()
+        modifies is
+        ensures
+            match ret
+                case Left(edks) =>
+                    && ValidEncryptedDataKeys(edks)
+                    // TODO: I think we need to establish freshness to connect
+                    //       deserialization with the caller.
+                    //       Times out.
+                    // && fresh(ReprEncryptedDataKeys(edks))
+                case Right(_)   => true
+        ensures is.Valid()
+    {
+        var res: Result;
+        var edkCount: uint16;
+        res := deserializeUnrestricted(is, 2);
+        match res {
+            case Left(bytes) => edkCount := arrayToUInt16(bytes);
+            case Right(e)    => return Right(e);
+        }
+
+        if edkCount == 0 {
+            return Right(DeserializationError("Encrypted data key count must be > 0."));
+        }
+
+        var edkEntries: array<EDKEntry> := new [edkCount];
+        var edks := EncryptedDataKeys(edkCount, edkEntries);
+        var i := 0;
+        while i < edkCount
+            invariant is.Valid()
+            invariant i <= edkCount
+            invariant InBoundsEncryptedDataKeysUpTo(edks.entries, i as nat)
+            // TODO: I think we need to establish freshness to connect
+            //       deserialization with the caller.
+            //       Times out.
+            //invariant fresh(ReprEncryptedDataKeysUpTo(edks.entries, i as nat))
+        {
+            // Key provider ID
+            var keyProviderIDLength: uint16;
+            res := deserializeUnrestricted(is, 2);
+            match res {
+                case Left(bytes) => keyProviderIDLength := arrayToUInt16(bytes);
+                case Right(e)    => return Right(e);
+            }
+
+            var keyProviderID := new uint8[keyProviderIDLength];
+            res := deserializeUTF8(is, keyProviderIDLength as nat);
+            match res {
+                case Left(bytes) => keyProviderID := bytes;
+                case Right(e)    => return Right(e);
+            }
+
+            // Key provider info
+            var keyProviderInfoLength: uint16;
+            res := deserializeUnrestricted(is, 2);
+            match res {
+                case Left(bytes) => keyProviderInfoLength := arrayToUInt16(bytes);
+                case Right(e)    => return Right(e);
+            }
+            
+            var keyProviderInfo := new uint8[keyProviderInfoLength];
+            res := deserializeUTF8(is, keyProviderInfoLength as nat);
+            match res {
+                case Left(bytes) => keyProviderInfo := bytes;
+                case Right(e)    => return Right(e);
+            }
+
+            // Encrypted data key
+            var edkLength: uint16;
+            res := deserializeUnrestricted(is, 2);
+            match res {
+                case Left(bytes) => edkLength := arrayToUInt16(bytes);
+                case Right(e)    => return Right(e);
+            }
+            
+            var edk := new uint8[edkLength];
+            res := deserializeUTF8(is, edkLength as nat);
+            match res {
+                case Left(bytes) => edk := bytes;
+                case Right(e)    => return Right(e);
+            }
+            
+            edks.entries[i] := EDKEntry(keyProviderID, keyProviderInfo, edk);
+            i := i + 1;
+        }
+
+        return Left(edks);
+    }
+
+    method deserializeContentType(is: StringReader) returns (ret: Result<T_ContentType>)
+        requires is.Valid()
+        modifies is
+        ensures is.Valid()
+    {
+        var res := readFixedLengthFromStreamOrFail(is, 1);
+        match res {
+            case Left(contentType) =>
+                if contentType[0] == 0x01 {
+                    return Left(NonFramed);
+                } else if contentType[0] == 0x02 {
+                    return Left(Framed);
+                } else {
+                    return Right(DeserializationError("Content type not supported."));
+                }
+            case Right(e) => return Right(e);
+        }
+    }
+
+    method deserializeReserved(is: StringReader) returns (ret: Result<T_Reserved>)
+        requires is.Valid()
+        modifies is
+        ensures is.Valid()
+    {
+        var res := readFixedLengthFromStreamOrFail(is, 4);
+        match res {
+            case Left(reserved) =>
+                if reserved[0] == reserved[1] == reserved[2] == reserved[3] == 0 {
+                    return Left(reserved[..]);
+                } else {
+                    return Right(DeserializationError("Reserved fields must be 0."));
+                }
+            case Right(e) => return Right(e);
+        }
+    }
+
+    method deserializeIVLength(is: StringReader, algSuiteId: AlgorithmSuite.ID) returns (ret: Result<uint8>)
+        requires is.Valid()
+        requires algSuiteId in AlgorithmSuite.Suite.Keys
+        modifies is
+        ensures
+            match ret
+                case Left(ivLength) => ValidIVLength(ivLength, algSuiteId)
+                case Right(_)       => true
+        ensures is.Valid()
+    {
+        var res := readFixedLengthFromStreamOrFail(is, 1);
+        match res {
+            case Left(ivLength) =>
+                if ivLength[0] == AlgorithmSuite.Suite[algSuiteId].params.ivLen {
+                    return Left(ivLength[0]);
+                } else {
+                    return Right(DeserializationError("Incorrect IV length."));
+                }
+            case Right(e) => return Right(e);
+        }
+    }
+
+    method deserializeFrameLength(is: StringReader, contentType: T_ContentType) returns (ret: Result<uint32>)
+        requires is.Valid()
+        modifies is
+        ensures
+            match ret
+                case Left(frameLength) => ValidFrameLength(frameLength, contentType)
+                case Right(_) => true
+        ensures is.Valid()
+    {
+        var res := readFixedLengthFromStreamOrFail(is, 4);
+        match res {
+            case Left(frameLength) =>
+                if contentType.NonFramed? && arrayToUInt32(frameLength) == 0 {
+                    return Left(arrayToUInt32(frameLength));
+                } else {
+                    return Right(DeserializationError("Frame length must be 0 when content type is non-framed."));
+                }
+            case Right(e) => return Right(e);
+        }
+    }
+    /**
+    * Reads raw header data from the input stream and populates the header with all of the information about the
+    * message.
+    */
+    method headerBody(is: StringReader) returns (ret: Result<HeaderBody>)
+        requires is.Valid()
+        modifies is
+        ensures is.Valid()
+        ensures
+            match ret
+                case Left(hb) =>
+                    && ValidHeaderBody(hb)
+                    // TODO: I think we need to establish freshness to connect
+                    //       deserialization with the caller.
+                    //       Times out.
+                    // && fresh(ReprAAD(hb.aad))
+                    // && fresh(ReprEncryptedDataKeys(hb.encryptedDataKeys))
+                case Right(_) => true
+    {
+        var version: T_Version;
+        {
+            var res := deserializeVersion(is);
+            match res {
+                case Left(version_) => version := version_;
+                case Right(e)       => return Right(e);
+            }
+        }
+
+        var typ: T_Type;
+        {
+            var res := deserializeType(is);
+            match res {
+                case Left(typ_) => typ := typ_;
+                case Right(e)   => return Right(e);
+            }
+        }
+        
+        var algorithmSuiteID: AlgorithmSuite.ID;
+        {
+            var res := deserializeAlgorithmSuiteID(is);
+            match res {
+                case Left(algorithmSuiteID_) => algorithmSuiteID := algorithmSuiteID_;
+                case Right(e)                => return Right(e);
+            }
+        }
+        
+        var messageID: T_MessageID;
+        {
+            var res := deserializeMsgID(is);
+            match res {
+                case Left(messageID_) => messageID := messageID_;
+                case Right(e)    => return Right(e);
+            }
+        }
+
+        // AAD deserialization:
+        var aad: T_AAD;
+        {
+            var res := deserializeAAD(is);
+            match res {
+                case Left(aad_) => aad := aad_;
+                case Right(e)   => return Right(e);
+            }
+        }
+
+        // EDK deserialization:
+        var encryptedDataKeys: T_EncryptedDataKeys;
+        {
+            var res := deserializeEncryptedDataKeys(is, aad);
+            match res {
+                case Left(encryptedDataKeys_) => encryptedDataKeys := encryptedDataKeys_;
+                case Right(e)   => return Right(e);
+            }
+        }
+
+        var contentType: T_ContentType;
+        {
+            var res := deserializeContentType(is);
+            match res {
+                case Left(contentType_) => contentType := contentType_;
+                case Right(e)           => return Right(e);
+            }
+        }
+        
+        var reserved: T_Reserved;
+        {
+            var res := deserializeReserved(is);
+            match res {
+                case Left(reserved_) => reserved := reserved_;
+                case Right(e)    => return Right(e);
+            }
+        }
+
+        var ivLength: uint8;
+        {
+            var res := deserializeIVLength(is, algorithmSuiteID);
+            match res {
+                case Left(ivLength_) => ivLength := ivLength_;
+                case Right(e)    => return Right(e);
+            }
+        }
+
+        var frameLength: uint32;
+        {
+            var res := deserializeFrameLength(is, contentType);
+            match res {
+                case Left(frameLength_) => frameLength := frameLength_;
+                case Right(e) => return Right(e);
+            }
+        }
+
+        ret := Left(
+                HeaderBody(
+                    version,
+                    typ,
+                    algorithmSuiteID,
+                    messageID,
+                    aad,
+                    encryptedDataKeys,
+                    contentType,
+                    reserved,
+                    ivLength,
+                    frameLength));
+    }
+
+    method deserializeAuthenticationTag(is: StringReader, tagLength: nat, ghost iv: array<uint8>) returns (ret: Result<array<uint8>>)
+        requires is.Valid()
+        modifies is
+        ensures
+            match ret
+                case Left(authenticationTag) => ValidAuthenticationTag(authenticationTag, tagLength, iv)
+                case Right(_) => true
+        ensures is.Valid()
+    {
+        ret := readFixedLengthFromStreamOrFail(is, tagLength);
+    }
+
+    method headerAuthentication(is: StringReader, body: HeaderBody) returns (ret: Result<HeaderAuthentication>)
+        requires is.Valid()
+        requires is.Repr !! ReprAAD(body.aad)
+        requires is.Repr !! ReprEncryptedDataKeys(body.encryptedDataKeys)
+        requires ReprAAD(body.aad) !! ReprEncryptedDataKeys(body.encryptedDataKeys)
+        requires body.algorithmSuiteID in AlgorithmSuite.Suite.Keys
+        modifies is
+        ensures unchanged(ReprAAD(body.aad))
+        ensures unchanged(ReprEncryptedDataKeys(body.encryptedDataKeys))
+        ensures is.Valid()
+        ensures
+            match ret
+                case Left(headerAuthentication) => ValidHeaderAuthentication(headerAuthentication, body.algorithmSuiteID)
+                case Right(_) => true
+    {
+        var iv: array<uint8>;
+        {
+            var res := deserializeUnrestricted(is, body.ivLength as nat);
+            match res {
+                case Left(bytes) => iv := bytes;
+                case Right(e)    => return Right(e);
+            }
+        }
+        
+        var authenticationTag: array<uint8>;
+        {
+            var res := deserializeAuthenticationTag(is, AlgorithmSuite.Suite[body.algorithmSuiteID].params.tagLen as nat, iv);
+            match res {
+                case Left(bytes) => authenticationTag := bytes;
+                case Right(e)    => return Right(e);
+            }
+        }
+        ret := Left(HeaderAuthentication(iv, authenticationTag));
+    }
+}
