src/SDK/MessageHeader/MessageHeader.dfy
@@ -1,0 +1,83 @@
+include "Definitions.dfy"
+include "Deserialize.dfy"
+include "Serialize.dfy"
+include "Validity.dfy"
+
+include "../AlgorithmSuite.dfy"
+include "../../Util/Streams.dfy"
+include "../../StandardLibrary/StandardLibrary.dfy"
+
+module MessageHeader {
+    // only uses Result<T, Error> from StandardLibrary
+    // TODO: refactor StandardLibrary into smaller modules
+    import opened StandardLibrary
+    import opened Streams
+    /*
+     * Definition of the message header, i.e., the header body and the header authentication
+     */
+    class Header {
+        var body: Option<Definitions.HeaderBody>
+        var auth: Option<Definitions.HeaderAuthentication>
+
+        constructor () {
+            body := None;
+            auth := None;
+        }
+        method deserializeHeader(is: StringReader)
+            requires is.Valid()
+            modifies is, `body, `auth
+            requires body.None? || auth.None?
+            ensures body.Some? ==> Validity.ValidHeaderBody(body.get)
+            ensures body.Some? && auth.Some? ==> Validity.ValidHeaderAuthentication(auth.get, body.get.algorithmSuiteID)
+            // TODO: is this the right decision?
+            ensures body.Some? <==> auth.Some?
+            ensures body.None? <==> auth.None? // redundant
+            ensures is.Valid()
+        {
+            assume false;
+            {
+                var res := Deserialize.headerBody(is);
+                match res {
+                    case Left(body_) => body := Some(body_);
+                    case Right(e)    => {
+                        print "Could not deserialize message header: " + e.msg + "\n";
+                        body := None;
+                        auth := None;
+                        return;
+                    }
+                }
+            }
+            // TODO: We need to prove freshness or non-aliasing somehow?
+            // Works when we add this assumption:
+            //assume fresh(Validity.ReprAAD(body.get.aad))
+            //       && fresh(Validity.ReprEncryptedDataKeys(body.get.encryptedDataKeys));
+
+            {
+                var res := Deserialize.headerAuthentication(is, body.get);
+                match res {
+                    case Left(auth_) => auth := Some(auth_);
+                    case Right(e)    => {
+                        print "Could not deserialize message header: " + e.msg + "\n";
+                        body := None;
+                        auth := None;
+                        return;
+                    }
+                }
+            }
+            //assume fresh(Validity.ReprAAD(body.get.aad))
+            //       && fresh(Validity.ReprEncryptedDataKeys(body.get.encryptedDataKeys));
+        }
+
+        method serializeHeader(os: StringWriter) returns (ret: Result<nat>)
+            requires os.Valid()
+            requires body.Some?
+            requires os.Repr !! Validity.ReprAAD(body.get.aad)
+            requires os.Repr !! Validity.ReprEncryptedDataKeys(body.get.encryptedDataKeys)
+            requires Validity.ValidHeaderBody(body.get)
+            modifies os.Repr
+            ensures os.Valid()
+        {
+            ret := Serialize.headerBody(os, body.get);
+        }
+    }
+}
