src/SDK/MessageHeader/Serialize.dfy
@@ -1,0 +1,176 @@
+include "Definitions.dfy"
+include "SerializeAAD.dfy"
+include "SerializeEDK.dfy"
+include "Validity.dfy"
+
+include "../../Util/Streams.dfy"
+include "../../StandardLibrary/StandardLibrary.dfy"
+
+module MessageHeader.Serialize {
+    import opened Definitions
+    import opened SerializeAAD
+    import opened SerializeEDK
+    import opened Validity
+    
+    import opened Streams
+    import opened StandardLibrary
+    import opened UInt = StandardLibrary.UInt
+    
+    function {:opaque} serialize(hb: HeaderBody): seq<uint8>
+        requires ValidHeaderBody(hb)
+        //requires ReprAAD(hb.aad) !! ReprEncryptedDataKeys(hb.encryptedDataKeys)
+        reads if hb.aad.AAD? then {hb.aad.kvPairs} else {}
+        reads ReprAAD(hb.aad)
+        reads ReprEncryptedDataKeys(hb.encryptedDataKeys)
+    {
+        reveal ValidHeaderBody();
+        [hb.version as uint8] + 
+        [hb.typ as uint8] + 
+        uint16ToSeq(hb.algorithmSuiteID as uint16) + 
+        hb.messageID + 
+        serializeAAD(hb.aad) + 
+        serializeEDK(hb.encryptedDataKeys) + 
+        (match hb.contentType case NonFramed => [0x01] case Framed => [0x02]) +
+        hb.reserved +
+        [hb.ivLength] +
+        uint32ToSeq(hb.frameLength)
+    }
+
+    method headerBody(os: StringWriter, hb: HeaderBody) returns (ret: Result<nat>)
+        requires os.Valid()
+        modifies os`data
+        requires ValidHeaderBody(hb)
+        // It's crucial to require no aliasing here
+        requires os.Repr !! ReprAAD(hb.aad)
+        requires os.Repr !! ReprEncryptedDataKeys(hb.encryptedDataKeys)
+        requires ReprAAD(hb.aad) !! ReprEncryptedDataKeys(hb.encryptedDataKeys)
+        ensures os.Valid()
+        // TODO: these should probably be enabled
+        //ensures unchanged(os`Repr)
+        //ensures unchanged(ReprAAD(hb.aad))
+        //ensures unchanged(ReprEncryptedDataKeys(hb.encryptedDataKeys))
+        //ensures old(|os.data|) <= |os.data|
+        ensures ValidHeaderBody(hb)
+        ensures
+            match ret
+                case Left(totalWritten) =>
+                    var serHb := (reveal serialize(); serialize(hb));
+                    var initLen := old(|os.data|);
+                    && totalWritten == |serHb|
+                    && initLen+totalWritten == |os.data|
+                    && serHb[..totalWritten] == os.data[initLen..initLen+totalWritten]
+                case Right(e) => true
+    {
+        var totalWritten := 0;
+        ghost var initLen := |os.data|;
+        reveal ValidHeaderBody();
+        reveal ValidAAD();
+        reveal ValidEncryptedDataKeys();
+        {
+            ret := os.WriteSingleByteSimple(hb.version as uint8);
+            match ret {
+                case Left(len) => totalWritten := totalWritten + len;
+                case Right(e)  => {
+                    return ret;
+                }
+            }
+        }
+
+        {
+            ret := os.WriteSingleByteSimple(hb.typ as uint8);
+            match ret {
+                case Left(len) => totalWritten := totalWritten + len;
+                case Right(e)  => {
+                    return ret;
+                }
+            }
+        }
+        
+        {
+            var bytes := uint16ToArray(hb.algorithmSuiteID as uint16);
+            ret := os.WriteSimple(bytes);
+            match ret {
+                case Left(len) => totalWritten := totalWritten + len;
+                case Right(e)  => {
+                    return ret;
+                }
+            }
+        }
+
+        {
+            ret := os.WriteSimpleSeq(hb.messageID);
+            match ret {
+                case Left(len) => totalWritten := totalWritten + len;
+                case Right(e)  => {
+                    return ret;
+                }
+            }
+        }
+
+        {
+            ret := serializeAADImpl(os, hb.aad);
+            match ret {
+                case Left(len) => totalWritten := totalWritten + len;
+                case Right(e)  => {
+                    return ret;
+                }
+            }
+        }
+        
+        {
+            ret := serializeEDKImpl(os, hb.encryptedDataKeys);
+            match ret {
+                case Left(len) => totalWritten := totalWritten + len;
+                case Right(e)  => return ret;
+            }
+        }
+
+        {
+            var contentType: uint8;
+            match hb.contentType {
+                case NonFramed => contentType := 0x01;
+                case Framed    => contentType := 0x02;
+            }
+            ret := os.WriteSingleByteSimple(contentType);
+            match ret {
+                case Left(len) =>
+                    totalWritten := totalWritten + len;
+                case Right(e)  =>
+                    return ret;
+            }
+        }
+
+        {
+            ret := os.WriteSimpleSeq(hb.reserved);
+            match ret {
+                case Left(len) => totalWritten := totalWritten + len;
+                case Right(e)  => return ret;
+            }
+        }
+
+        {
+            ret := os.WriteSingleByteSimple(hb.ivLength);
+            match ret {
+                case Left(len) => totalWritten := totalWritten + len;
+                case Right(e)  => return ret;
+            }
+        }
+        
+        {
+            var bytes := uint32ToArray(hb.frameLength);
+            ret := os.WriteSimple(bytes);
+            match ret {
+                case Left(len) => totalWritten := totalWritten + len;
+                case Right(e)  => return ret;
+            }
+        }
+        assert ValidHeaderBody(hb);
+        reveal serialize();
+        ghost var serHb := serialize(hb);
+        assert totalWritten == |serHb|;
+        assert initLen+totalWritten == |os.data|;
+        assert serHb[..totalWritten] == os.data[initLen..initLen+totalWritten];
+
+        return Left(totalWritten);
+    }
+}
