src/SDK/MessageHeader/SerializeAAD.dfy
@@ -1,0 +1,190 @@
+include "Definitions.dfy"
+include "Validity.dfy"
+
+include "../../Util/Streams.dfy"
+include "../../StandardLibrary/StandardLibrary.dfy"
+
+module MessageHeader.SerializeAAD {
+    import opened Definitions
+    import opened Validity
+    
+    import opened Streams
+    import opened StandardLibrary
+    import opened UInt = StandardLibrary.UInt
+
+    function encCtxToSeq(kvPairs: EncCtx, i: nat): seq<uint8>
+        requires forall i :: 0 <= i < kvPairs.Length ==> kvPairs[i].0.Length <= UINT16_MAX && kvPairs[i].1.Length <= UINT16_MAX
+        decreases kvPairs.Length - i
+        reads kvPairs
+        reads set i | 0 <= i < kvPairs.Length :: kvPairs[i].0
+        reads set i | 0 <= i < kvPairs.Length :: kvPairs[i].1
+        // reads ReprAADUpTo(kvPairs, kvPairs.Length)
+    {
+        if i < kvPairs.Length
+        then 
+            uint16ToSeq(kvPairs[i].0.Length as uint16) + kvPairs[i].0[..] +
+            uint16ToSeq(kvPairs[i].1.Length as uint16) + kvPairs[i].1[..] +
+            encCtxToSeq(kvPairs, i + 1)
+        else []
+    }
+
+    function serializeAAD(aad: T_AAD): seq<uint8>
+        requires ValidAAD(aad)
+        reads ReprAAD(aad)
+    {
+        match aad {
+            case AAD(length, kvPairs) =>
+                uint16ToSeq(length) +
+                // It would be nicer if this could be a flatten + map as for AAD
+                uint16ToSeq(kvPairs.Length as uint16) + encCtxToSeq(kvPairs, 0)
+            case EmptyAAD() =>
+                uint16ToSeq(0)
+        }
+    }
+    
+    method serializeAADImpl(os: StringWriter, aad: T_AAD) returns (ret: Result<nat>)
+        requires os.Valid()
+        modifies os`data // do we need to establish non-aliasing with encryptedDataKeys here?
+        ensures os.Valid()
+        requires ValidAAD(aad)
+        requires os.Repr !! ReprAAD(aad)
+        ensures ValidAAD(aad)
+        ensures unchanged(os`Repr)
+        ensures unchanged(ReprAAD(aad))
+        //ensures old(|os.data|) <= |os.data|
+        ensures
+            match ret
+                case Left(totalWritten) =>
+                    var serAAD := serializeAAD(aad);
+                    var initLen := old(|os.data|);
+                    && totalWritten == |serAAD|
+                    && initLen+totalWritten == |os.data|
+                    && os.data == old(os.data + serAAD)
+                case Right(e) => true
+    {
+        var totalWritten := 0;
+        ghost var initLen := |os.data|;
+        ghost var written: seq<nat> := [initLen];
+        ghost var i := 0;
+
+        match aad {
+            case AAD(length, kvPairs) => {
+                {
+                    // Key Value Pairs Length (number of bytes of total AAD)
+                    var bytes := uint16ToArray(length);
+                    ret := os.WriteSimple(bytes);
+                    match ret {
+                        case Left(len) => totalWritten := totalWritten + len;
+                        case Right(e)  => return ret;
+                    }
+                    i := i + 1;
+                    written := written + [initLen + totalWritten];
+                    assert written[i] - written[i-1] == bytes.Length;
+                    assert written[i-1] <= written[i] <= |os.data| ==> os.data[written[i-1]..written[i]] == bytes[..];
+                    assert totalWritten <= |serializeAAD(aad)|;
+                }
+
+                assert 0 < length;
+                assert 0 < kvPairs.Length;
+                {
+                    assert InBoundsKVPairs(kvPairs) ==> kvPairs.Length <= UINT16_MAX;
+                    // Key Value Pair Count (number of key value pairs)
+                    var bytes := uint16ToArray(kvPairs.Length as uint16);
+                    ret := os.WriteSimple(bytes);
+                    match ret {
+                        case Left(len) => totalWritten := totalWritten + len;
+                        case Right(e)  => return ret;
+                    }
+                    i := i + 1;
+                    written := written + [initLen + totalWritten];
+                    assert written[i] - written[i-1] == bytes.Length;
+                    assert written[i-1] <= written[i] <= |os.data| ==> os.data[written[i-1]..written[i]] == bytes[..];
+                    assert totalWritten <= |serializeAAD(aad)|;
+                }
+            
+                assume false; // TODO: verification times out after this point. I believe that we just do too many heap updates.
+
+                var j := 0;
+                while j < kvPairs.Length
+                    invariant j <= kvPairs.Length
+                    invariant os.Repr !! ReprAAD(aad)
+                    invariant unchanged(os`Repr)
+                    invariant InBoundsKVPairsUpTo(kvPairs, j)
+                    invariant ValidAAD(aad)
+                    invariant totalWritten <= |serializeAAD(aad)|
+                    invariant initLen+totalWritten <= |os.data|
+                    invariant serializeAAD(aad)[written[i-1]-initLen..written[i]-initLen] == os.data[written[i-1]..written[i]];
+                    //invariant serializeAAD(aad)[..totalWritten] == os.data[initLen..written[i]];
+                {
+                    {
+                        assert InBoundsKVPairsUpTo(kvPairs, j) ==> kvPairs[j].0.Length <= UINT16_MAX;
+                        var bytes := uint16ToArray(kvPairs[j].0.Length as uint16);
+                        ret := os.WriteSimple(bytes);
+                        match ret {
+                            case Left(len) => totalWritten := totalWritten + len;
+                            case Right(e)  => return ret;
+                        }
+                        i := i + 1;
+                        written := written + [initLen + totalWritten];
+                        assert written[i] - written[i-1] == bytes.Length;
+                        assert written[i-1] <= written[i] <= |os.data| ==> os.data[written[i-1]..written[i]] == bytes[..];
+                    }
+
+                    {
+                        var bytes := kvPairs[j].0;
+                        ret := os.WriteSimple(bytes);
+                        match ret {
+                            case Left(len) => totalWritten := totalWritten + len;
+                            case Right(e)  => return ret;
+                        }
+                        i := i + 1;
+                        written := written + [initLen + totalWritten];
+                        assert written[i] - written[i-1] == bytes.Length;
+                        assert written[i-1] <= written[i] <= |os.data| ==> os.data[written[i-1]..written[i]] == bytes[..];
+                    }
+                    
+                    {
+                        assert InBoundsKVPairsUpTo(kvPairs, j) ==> kvPairs[j].1.Length <= UINT16_MAX;
+                        var bytes := uint16ToArray(kvPairs[j].1.Length as uint16);
+                        ret := os.WriteSimple(bytes);
+                        match ret {
+                            case Left(len) => totalWritten := totalWritten + len;
+                            case Right(e)  => return ret;
+                        }
+                        i := i + 1;
+                        written := written + [initLen + totalWritten];
+                        assert written[i] - written[i-1] == bytes.Length;
+                        assert written[i-1] <= written[i] <= |os.data| ==> os.data[written[i-1]..written[i]] == bytes[..];
+                    }
+                    
+                    {
+                        var bytes := kvPairs[j].1;
+                        ret := os.WriteSimple(bytes);
+                        match ret {
+                            case Left(len) => totalWritten := totalWritten + len;
+                            case Right(e)  => return ret;
+                        }
+                        i := i + 1;
+                        written := written + [initLen + totalWritten];
+                        assert written[i] - written[i-1] == bytes.Length;
+                        assert written[i-1] <= written[i] <= |os.data| ==> os.data[written[i-1]..written[i]] == bytes[..];
+                    }
+                    j := j + 1;
+                }
+            }
+            case EmptyAAD() => {
+                var bytes := uint16ToArray(0);
+                ret := os.WriteSimple(bytes);
+                match ret {
+                    case Left(len) => totalWritten := totalWritten + len;
+                    case Right(e)  => return ret;
+                }
+                i := i + 1;
+                written := written + [initLen + totalWritten];
+                assert written[i] - written[i-1] == 2;
+                assert written[i-1] <= written[i] <= |os.data| ==> os.data[written[i-1]..written[i]] == bytes[..];
+
+            }
+        }
+    }
+}
