src/SDK/MessageHeader/SerializeEDK.dfy
@@ -1,0 +1,178 @@
+include "Definitions.dfy"
+include "Validity.dfy"
+
+include "../../Util/Streams.dfy"
+include "../../StandardLibrary/StandardLibrary.dfy"
+
+module MessageHeader.SerializeEDK {
+    import opened Definitions
+    import opened Validity
+    
+    import opened Streams
+    import opened StandardLibrary
+    import opened UInt = StandardLibrary.UInt
+
+    // Alternative w/o flatten/map
+    function serializeEDKEntries(entries: seq<EDKEntry>): seq<uint8>
+        requires forall i :: 0 <= i < |entries| ==>
+            && entries[i].keyProviderId.Length   <= UINT16_MAX
+            && entries[i].keyProviderInfo.Length <= UINT16_MAX
+            && entries[i].encDataKey.Length      <= UINT16_MAX
+        reads ReprEncryptedDataKeysUpTo(entries, |entries|)
+    {
+        if entries == []
+        then []
+        else
+            var entry := entries[0];
+            uint16ToSeq(entry.keyProviderId.Length as uint16)   + entry.keyProviderId[..] +
+            uint16ToSeq(entry.keyProviderInfo.Length as uint16) + entry.keyProviderInfo[..] +
+            uint16ToSeq(entry.encDataKey.Length as uint16)      + entry.encDataKey[..] +
+            serializeEDKEntries(entries[1..])
+    }
+
+    function serializeEDK(encryptedDataKeys: T_EncryptedDataKeys): seq<uint8>
+        requires ValidEncryptedDataKeys(encryptedDataKeys)
+        reads ReprEncryptedDataKeys(encryptedDataKeys)
+    {
+        uint16ToSeq(encryptedDataKeys.count) +
+        serializeEDKEntries(encryptedDataKeys.entries[..])
+    }
+
+    method serializeEDKImpl(os: StringWriter, encryptedDataKeys: T_EncryptedDataKeys) returns (ret: Result<nat>)
+        requires os.Valid()
+        modifies os`data
+        ensures os.Valid()
+        requires ValidEncryptedDataKeys(encryptedDataKeys)
+        requires os.Repr !! ReprEncryptedDataKeys(encryptedDataKeys)
+        ensures ValidEncryptedDataKeys(encryptedDataKeys)
+        ensures unchanged(os`Repr)
+        ensures unchanged(ReprEncryptedDataKeys(encryptedDataKeys))
+        //ensures old(|os.data|) <= |os.data|
+        ensures
+            match ret
+                case Left(totalWritten) =>
+                    var serEDK := serializeEDK(encryptedDataKeys);
+                    var initLen := old(|os.data|);
+                    && totalWritten == |serEDK|
+                    && initLen+totalWritten == |os.data|
+                    && os.data == old(os.data + serEDK)
+                case Right(e) => true
+    {
+        var totalWritten: nat := 0;
+        ghost var initLen := |os.data|;
+        ghost var prevPos: nat := initLen;
+        ghost var currPos: nat := initLen;
+
+        {
+            var bytes := uint16ToArray(encryptedDataKeys.count as uint16);
+            ret := os.WriteSimple(bytes);
+            match ret {
+                case Left(len) => totalWritten := totalWritten + len;
+                case Right(e)  => return ret;
+            }
+            prevPos := currPos;
+            currPos := initLen + totalWritten;
+            assert currPos - prevPos == bytes.Length;
+            assert prevPos <= currPos <= |os.data| ==> os.data[prevPos..currPos] == bytes[..];
+            assert totalWritten <= |serializeEDK(encryptedDataKeys)|;
+        }
+        assume false;
+
+        var j := 0;
+        ghost var written: seq<nat> := [currPos, currPos];
+        while j < encryptedDataKeys.entries.Length
+            invariant j <= encryptedDataKeys.entries.Length
+            invariant j < |written|
+            invariant os.Repr !! ReprEncryptedDataKeys(encryptedDataKeys)
+            invariant unchanged(os`Repr)
+            invariant InBoundsEncryptedDataKeysUpTo(encryptedDataKeys.entries, j)
+            invariant ValidEncryptedDataKeys(encryptedDataKeys)
+            invariant initLen + totalWritten == currPos
+            invariant 0 <= initLen <= prevPos <= currPos <= |os.data|
+            invariant currPos-initLen <= |serializeEDK(encryptedDataKeys)|
+            invariant serializeEDK(encryptedDataKeys)[..currPos-initLen] == os.data[initLen..currPos]
+            invariant serializeEDK(encryptedDataKeys)[prevPos-initLen..currPos-initLen] == os.data[prevPos..currPos];
+            invariant 1 <= j ==> os.data[initLen..written[j]] == os.data[initLen..written[j-1]] + serializeEDKEntries(encryptedDataKeys.entries[..j])
+        {
+            var entry := encryptedDataKeys.entries[j];
+            {
+                var bytes := uint16ToArray(entry.keyProviderId.Length as uint16);
+                ret := os.WriteSimple(bytes);
+                match ret {
+                    case Left(len) => totalWritten := totalWritten + len;
+                    case Right(e)  => return ret;
+                }
+                prevPos := currPos;
+                currPos := initLen + totalWritten;
+                assert prevPos <= currPos <= |os.data| ==> os.data[prevPos..currPos] == bytes[..];
+            }
+
+            {
+                var bytes := entry.keyProviderId;
+                ret := os.WriteSimple(bytes);
+                match ret {
+                    case Left(len) => totalWritten := totalWritten + len;
+                    case Right(e)  => return ret;
+                }
+                prevPos := currPos;
+                currPos := initLen + totalWritten;
+                assert currPos - prevPos == bytes.Length;
+                assert prevPos <= currPos <= |os.data| ==> os.data[prevPos..currPos] == bytes[..];
+            }
+
+            {
+                var bytes := uint16ToArray(entry.keyProviderInfo.Length as uint16);
+                ret := os.WriteSimple(bytes);
+                match ret {
+                    case Left(len) => totalWritten := totalWritten + len;
+                    case Right(e)  => return ret;
+                }
+                prevPos := currPos;
+                currPos := initLen + totalWritten;
+                assert currPos - prevPos == bytes.Length;
+                assert prevPos <= currPos <= |os.data| ==> os.data[prevPos..currPos] == bytes[..];
+            }
+
+            {
+                var bytes := entry.keyProviderInfo;
+                ret := os.WriteSimple(bytes);
+                match ret {
+                    case Left(len) => totalWritten := totalWritten + len;
+                    case Right(e)  => return ret;
+                }
+                prevPos := currPos;
+                currPos := initLen + totalWritten;
+                assert currPos - prevPos == bytes.Length;
+                assert prevPos <= currPos <= |os.data| ==> os.data[prevPos..currPos] == bytes[..];
+            }
+
+            {
+                var bytes := uint16ToArray(entry.encDataKey.Length as uint16);
+                ret := os.WriteSimple(bytes);
+                match ret {
+                    case Left(len) => totalWritten := totalWritten + len;
+                    case Right(e)  => return ret;
+                }
+                prevPos := currPos;
+                currPos := initLen + totalWritten;
+                assert currPos - prevPos == bytes.Length;
+                assert prevPos <= currPos <= |os.data| ==> os.data[prevPos..currPos] == bytes[..];
+            }
+
+            {
+                var bytes := entry.encDataKey;
+                ret := os.WriteSimple(bytes);
+                match ret {
+                    case Left(len) => totalWritten := totalWritten + len;
+                    case Right(e)  => return ret;
+                }
+                prevPos := currPos;
+                currPos := initLen + totalWritten;
+                assert currPos - prevPos == bytes.Length;
+                assert prevPos <= currPos <= |os.data| ==> os.data[prevPos..currPos] == bytes[..];
+            }
+            written := written + [currPos];
+            j := j + 1;
+        }
+    }
+}
